added a generalized version of the dependency generator and some example stuffs

src/DependencyGenerator.v
@@ -1,40 +1,389 @@
-(* This takes a datalog program, and for every rule, it generates the rules that it might depend on *)
+(* This takes a datalog program, and for every rule, it generates the rules that it might depend on
+   which will then be fed into gurobi to find an optimal layout. *)
+
 From Datalog Require Import Datalog.
 From Stdlib Require Import List.
 From Stdlib Require Import String.
+From Stdlib Require Import Bool.Bool.
 Import ListNotations.
-
-
-(* Then, it will try to generate a layout for the program which can be fed into gurobi *)
+Open Scope bool_scope.
+Open Scope string_scope.
 
 Definition rel := string.
 Definition var := string.
 Definition fn := string.
 Definition aggregator := unit.
-Definition T := nat.  (* semantic domain for interpretation *)
+Definition T := string.  (* semantic domain for interpretation *)
 Definition rule := Datalog.rule rel var fn aggregator.
 Definition program := list rule.
+Definition expr := Datalog.expr var fn.
+Definition fact := Datalog.fact rel var fn.
+
+(* Basic Utilities *)
+
+Definition is_var (e : expr) : bool :=
+  match e with
+  | Datalog.var_expr _ => true
+  | _ => false
+  end.
+
+Definition is_const (e : expr) : bool :=
+  match e with
+  | Datalog.fun_expr _ [] => true
+  | _ => false
+  end.
+
+Definition is_fun_app (e : expr) : bool :=
+  match e with
+  | Datalog.fun_expr _ (_::_) => true
+  | _ => false
+  end.
+
+Definition get_var (e : expr) : option var :=
+  match e with
+  | Datalog.var_expr v => Some v
+  | _ => None
+  end.
+
+Definition get_const (e : expr) : option fn :=
+  match e with
+  | Datalog.fun_expr f [] => Some f
+  | _ => None
+  end.
+
+(* Subst *)
+
+Definition subst_env := list (var * expr).
+
+Definition lookup_subst (env : subst_env) (v : var) : option expr :=
+  match List.find (fun p => String.eqb (fst p) v) env with
+  | Some (_, e) => Some e
+  | None => None
+  end.
+
+Fixpoint do_expr_subst (env : subst_env) (e : expr) : expr :=
+  match e with
+  | Datalog.var_expr v =>
+      match lookup_subst env v with
+      | Some e' => e'
+      | None => e
+      end
+  | Datalog.fun_expr f args =>
+      Datalog.fun_expr f (map (do_expr_subst env) args)
+  end.
 
 
-(* For every rule we want the transitive closure of its dependencies. Given a program, 
-   we want to be able to get all the rules that could possibly generate conclusions that
-   would be used in hypotheses *)
+(* Eqb *)
+Fixpoint list_eqb {A : Type} (eqb : A -> A -> bool) (l1 l2 : list A) : bool :=
+  match l1, l2 with
+  | [], [] => true
+  | x :: xs, y :: ys => eqb x y && list_eqb eqb xs ys
+  | _, _ => false
+  end.
+
+Fixpoint expr_eqb (e1 e2 : expr) : bool :=
+  match e1, e2 with
+  | Datalog.var_expr _, Datalog.var_expr _ =>
+      true
+      (* XXX: need to handle alpha equivalence here *)
+  | Datalog.var_expr _, Datalog.fun_expr _ [] =>
+      true
+  | Datalog.fun_expr _ [], Datalog.var_expr _ =>
+      true
+  | Datalog.fun_expr f1 args1, Datalog.fun_expr f2 args2 =>
+      String.eqb f1 f2 &&
+      (fix expr_list_eqb (l1 l2 : list expr) : bool :=
+         match l1, l2 with
+         | [], [] => true
+         | x1 :: t1, x2 :: t2 =>
+             expr_eqb x1 x2 && expr_list_eqb t1 t2
+         | _, _ => false
+         end) args1 args2
+  | _, _ => false
+  end.
+
+(* Collect *)
+Fixpoint collect_vars (e : expr) : list var :=
+  match e with
+  | Datalog.var_expr v => [v]
+  | Datalog.fun_expr _ args => 
+      flat_map collect_vars args
+  end.
+
+Fixpoint collect_consts (e : expr) : list fn :=
+  match e with
+  | Datalog.var_expr _ => []
+  | Datalog.fun_expr f [] => [f]
+  | Datalog.fun_expr _ args => 
+      flat_map collect_consts args
+  end.
+
+Fixpoint collect_funs (e : expr) : list fn :=
+  match e with
+  | Datalog.var_expr _ => []
+  | Datalog.fun_expr f args => 
+      f :: flat_map collect_funs args
+  end.
+
+(* Collect Fact *)
+
+Definition collect_vars_from_fact (f : fact) : list var :=
+  flat_map collect_vars (Datalog.fact_args f).
+
+Definition collect_consts_from_fact (f : fact) : list fn :=
+  flat_map collect_consts (Datalog.fact_args f).
+
+Definition collect_funs_from_fact (f : fact) : list fn :=
+  flat_map collect_funs (Datalog.fact_args f).
+
+Definition is_abstract (f : fact) : bool :=
+  forallb is_var (Datalog.fact_args f).
+
+Definition is_grounded_fact (f : fact) : bool :=
+  forallb is_const (Datalog.fact_args f).
+
+(* Collect for Rules *)
+
+Definition collect_vars_from_hyps (r : rule) : list var :=
+  flat_map collect_vars_from_fact (Datalog.rule_hyps r).
+
+Definition collect_vars_from_concls (r : rule) : list var :=
+  flat_map collect_vars_from_fact (Datalog.rule_concls r).
+
+Definition collect_vars_from_rule (r : rule) : list var :=
+  collect_vars_from_hyps r ++ collect_vars_from_concls r.
+
+Definition collect_consts_from_hyps (r : rule) : list fn :=
+  flat_map collect_consts_from_fact (Datalog.rule_hyps r).
+
+Definition collect_consts_from_concls (r : rule) : list fn :=
+  flat_map collect_consts_from_fact (Datalog.rule_concls r).
+
+Definition collect_consts_from_rule (r : rule) : list fn :=
+  collect_consts_from_hyps r ++ collect_consts_from_concls r.
+
+Definition collect_funs_from_hyps (r : rule) : list fn :=
+  flat_map collect_funs_from_fact (Datalog.rule_hyps r).
+
+Definition collect_funs_from_concls (r : rule) : list fn :=
+  flat_map collect_funs_from_fact (Datalog.rule_concls r).
+
+Definition collect_funs_from_rule (r : rule) : list fn :=
+  collect_funs_from_hyps r ++ collect_funs_from_concls r.
 
 Definition get_rule_concls_rels (r : rule) : list rel :=
   map (fun fact => Datalog.fact_R fact) (Datalog.rule_concls r).
 
-
 Definition get_rule_hyps_rels (r : rule) : list rel :=
   map (fun fact => Datalog.fact_R fact) (Datalog.rule_hyps r).
 
+(* Pattern Matching *)
 
-(* We want to get every single rule that generates conclusions that the hypotheses might depend on *)
-Definition get_directly_dependent_rules (p : program) (r : rule) : program :=
-  filter (fun r' => 
-            let conc_rels := get_rule_concls_rels r' in
-            let hyp_rels := get_rule_hyps_rels r in
-            existsb (fun rel => existsb (String.eqb rel) conc_rels) hyp_rels)
-         p.
+Definition facts_compatible (f1 f2 : fact) : bool :=
+  String.eqb (Datalog.fact_R f1) (Datalog.fact_R f2) &&
+  list_eqb expr_eqb (Datalog.fact_args f1) (Datalog.fact_args f2).
 
-Compute (get_directly_dependent_rules [] ({| Datalog.rule_hyps := []; Datalog.rule_concls := [] |})).
+Definition conc_matches_hyp (conc hyp : fact) : bool :=
+  facts_compatible conc hyp.
 
+Definition rule_concls_match_hyps (r1 r2 : rule) : bool :=
+  existsb (fun conc => 
+    existsb (fun hyp => conc_matches_hyp conc hyp) (Datalog.rule_hyps r2)
+  ) (Datalog.rule_concls r1).
+
+Definition rule_depends_on (r1 r2 : rule) : bool :=
+  rule_concls_match_hyps r1 r2.
+
+Definition get_rule_dependencies (p : program) (r : rule) : program :=
+  filter (fun r' => rule_depends_on r' r) p.
+
+Definition get_rules_dependent_on (p : program) (r : rule) : program :=
+  filter (fun r' => rule_depends_on r r') p.
+
+(* Examples! *)
+
+Definition x_var : expr := Datalog.var_expr "x".
+Definition y_var : expr := Datalog.var_expr "y".
+
+Definition const_42 : expr := Datalog.fun_expr "42" [].
+Definition const_hello : expr := Datalog.fun_expr "hello" [].
+
+Definition add_expr : expr := Datalog.fun_expr "add" [x_var; const_42].
+
+(* Test is_var *)
+Check is_var x_var : bool.
+Goal is_var x_var = true. Proof. reflexivity. Qed.
+
+Check is_var const_42 : bool.
+Goal is_var const_42 = false. Proof. reflexivity. Qed.
+
+Check is_var add_expr : bool.
+Goal is_var add_expr = false. Proof. reflexivity. Qed.
+
+(* Test is_const *)
+Check is_const x_var : bool.
+Goal is_const x_var = false. Proof. reflexivity. Qed.
+
+Check is_const const_42 : bool.
+Goal is_const const_42 = true. Proof. reflexivity. Qed.
+
+Check is_const add_expr : bool.
+Goal is_const add_expr = false. Proof. reflexivity. Qed.
+
+(* Test get_var *)
+Check get_var x_var : option var.
+Goal get_var x_var = Some "x". Proof. reflexivity. Qed.
+
+Check get_var const_42 : option var.
+Goal get_var const_42 = None. Proof. reflexivity. Qed.
+
+(* Test get_const *)
+Check get_const const_42 : option fn.
+Goal get_const const_42 = Some "42". Proof. reflexivity. Qed.
+
+Check get_const x_var : option fn.
+Goal get_const x_var = None. Proof. reflexivity. Qed.
+
+(* Test collect_vars *)
+Check collect_vars add_expr : list var.
+Goal collect_vars add_expr = ["x"]. Proof. reflexivity. Qed.
+
+(* Test collect_consts *)
+Check collect_consts add_expr : list fn.
+Goal collect_consts add_expr = ["42"]. Proof. reflexivity. Qed.
+
+(* Example fact with mixed variables and constants *)
+Definition example_fact : fact :=
+  {| Datalog.fact_R := "edge";
+     Datalog.fact_args := [x_var; const_42; y_var] |}.
+
+Check collect_vars_from_fact example_fact : list var.
+Goal collect_vars_from_fact example_fact = ["x"; "y"]. Proof. reflexivity. Qed.
+
+Check collect_consts_from_fact example_fact : list fn.
+Goal collect_consts_from_fact example_fact = ["42"]. Proof. reflexivity. Qed.
+
+(* ========== Examples: Alpha Equivalence ========== *)
+
+(* Create test rules for alpha equivalence *)
+Definition rule1 : rule :=
+  {| rule_agg := None;
+     rule_hyps := [
+       {| fact_R := "A"; fact_args := [x_var; y_var] |}
+     ];
+     rule_concls := [
+       {| fact_R := "B"; fact_args := [x_var; y_var] |}
+     ] |}.
+
+Definition rule2 : rule :=
+  {| rule_agg := None;
+     rule_hyps := [
+       {| fact_R := "A"; fact_args := [const_42; y_var] |}
+     ];
+     rule_concls := [
+       {| fact_R := "B"; fact_args := [const_42; y_var] |}
+     ] |}.
+
+Definition rule3 : rule :=
+  {| rule_agg := None;
+     rule_hyps := [
+       {| fact_R := "A"; fact_args := [x_var; y_var] |}
+     ];
+     rule_concls := [
+       {| fact_R := "B"; fact_args := [x_var; y_var] |}
+     ] |}.
+
+Definition rule4 : rule :=
+  {| rule_agg := None;
+     rule_hyps := [
+       {| fact_R := "A"; fact_args := [x_var] |}
+     ];
+     rule_concls := [
+       {| fact_R := "B"; fact_args := [x_var; y_var] |}
+     ] |}.
+
+(* Test matching constants *)
+Check facts_compatible 
+  {| fact_R := "A"; fact_args := [x_var; y_var] |}
+  {| fact_R := "edge"; fact_args := [const_42; y_var] |} : bool.
+Goal facts_compatible 
+  {| fact_R := "edge"; fact_args := [x_var; y_var] |}
+  {| fact_R := "edge"; fact_args := [const_42; y_var] |} = true. 
+Proof. reflexivity. Qed.
+
+Check facts_compatible 
+  {| fact_R := "edge"; fact_args := [const_42; y_var] |}
+  {| fact_R := "edge"; fact_args := [const_hello; y_var] |} : bool.
+Goal facts_compatible 
+  {| fact_R := "edge"; fact_args := [const_42; y_var] |}
+  {| fact_R := "edge"; fact_args := [const_hello; y_var] |} = false. 
+Proof. reflexivity. Qed.
+
+(* Test rule-level dependency *)
+Check rule_depends_on rule1 rule2 : bool.
+Goal rule_depends_on rule1 rule2 = false. Proof. reflexivity. Qed.
+
+Check rule_depends_on rule2 rule1 : bool.
+Goal rule_depends_on rule2 rule1 = false. Proof. reflexivity. Qed.
+
+Check rule_depends_on rule1 rule4 : bool.
+Goal rule_depends_on rule1 rule4 = false. Proof. reflexivity. Qed.
+
+(* Test dependency finding *)
+Definition test_program : program := [rule1; rule2; rule3; rule4].
+
+Check get_rule_dependencies test_program rule2 : program.
+Goal get_rule_dependencies test_program rule2 = []. Proof. reflexivity. Qed.
+
+Check get_rules_dependent_on test_program rule1 : program.
+Goal get_rules_dependent_on test_program rule1 = []. Proof. reflexivity. Qed.
+
+Definition fact_edge_xy : fact :=
+  {| fact_R := "A"; fact_args := [x_var; y_var] |}.
+
+Definition fact_edge_42y : fact :=
+  {| fact_R := "A"; fact_args := [const_42; y_var] |}.
+
+Check facts_compatible fact_edge_xy fact_edge_42y : bool.
+Goal facts_compatible fact_edge_xy fact_edge_42y = true. Proof. reflexivity. Qed.
+
+Definition fact1 : fact :=
+  {| Datalog.fact_R := "A";
+     Datalog.fact_args := [x_var; y_var] |}.
+
+Definition fact2 : fact :=
+  {| Datalog.fact_R := "A";
+     Datalog.fact_args := [const_42; y_var] |}.
+
+Definition fact3 : fact :=
+  {| Datalog.fact_R := "A";
+     Datalog.fact_args := [const_42; const_hello] |}.
+
+Definition fact4 : fact :=
+  {| Datalog.fact_R := "B";
+     Datalog.fact_args := [x_var; y_var] |}.
+
+Check facts_compatible fact1 fact2 : bool.
+Goal facts_compatible fact1 fact2 = true. Proof. reflexivity. Qed.
+
+Check facts_compatible fact1 fact3 : bool.
+Goal facts_compatible fact1 fact3 = true. Proof. reflexivity. Qed.
+
+Check facts_compatible fact2 fact3 : bool.
+Goal facts_compatible fact2 fact3 = true. Proof. reflexivity. Qed.
+
+Check facts_compatible fact1 fact4 : bool.
+Goal facts_compatible fact1 fact4 = false. Proof. reflexivity. Qed.
+
+Check expr_eqb x_var (Datalog.var_expr "x") : bool.
+Goal expr_eqb x_var (Datalog.var_expr "x") = true. Proof. reflexivity. Qed.
+
+Check expr_eqb x_var y_var : bool.
+Goal expr_eqb x_var y_var = true. Proof. reflexivity. Qed.
+
+Check expr_eqb const_42 (Datalog.fun_expr "42" []) : bool.
+Goal expr_eqb const_42 (Datalog.fun_expr "42" []) = true. Proof. reflexivity. Qed.
+
+Check expr_eqb const_42 const_hello : bool.
+
+Goal expr_eqb const_42 const_hello = false. Proof. reflexivity. Qed.
