src/Family.v
@@ -1,0 +1,88 @@
+From Stdlib Require Import Strings.String.
+From Datalog Require Import Datalog.
+From Stdlib Require Import List.
+From Datalog Require Import FancyNotations.
+From DatalogRocq Require Import DependencyGenerator.
+Import ListNotations.
+Open Scope string_scope.
+
+
+Definition const (c : fn) : expr := fun_expr c [].
+Definition var (x : var) : expr := var_expr x.
+
+Definition r_parent_anna : rule :=
+  {| rule_agg := None;
+     rule_hyps := [];
+     rule_concls := [
+       {| fact_R := "parent"; fact_args := [const "Anna"; const "Bob"] |}
+     ] |}.
+
+Definition r_ancestor1 : rule :=
+  {| rule_agg := None;
+     rule_hyps := [
+       {| fact_R := "parent"; fact_args := [var "x"; var "y"] |}
+     ];
+     rule_concls := [
+       {| fact_R := "ancestor"; fact_args := [var "x"; var "y"] |}
+     ] |}.
+
+Definition r_ancestor2 : rule :=
+  {| rule_agg := None;
+     rule_hyps := [
+       {| fact_R := "parent"; fact_args := [var "x"; var "z"] |};
+       {| fact_R := "ancestor"; fact_args := [var "z"; var "y"] |}
+     ];
+     rule_concls := [
+       {| fact_R := "ancestor"; fact_args := [var "x"; var "y"] |}
+     ] |}.
+
+Definition r_sibling : rule :=
+  {| rule_agg := None;
+     rule_hyps := [
+       {| fact_R := "parent"; fact_args := [var "p"; var "x"] |};
+       {| fact_R := "parent"; fact_args := [var "p"; var "y"] |}
+     ];
+     rule_concls := [
+       {| fact_R := "sibling"; fact_args := [var "x"; var "y"] |}
+     ] |}.
+
+Definition r_aunt_uncle : rule :=
+  {| rule_agg := None;
+     rule_hyps := [
+       {| fact_R := "sibling"; fact_args := [var "x"; var "p"] |};
+       {| fact_R := "parent"; fact_args := [var "p"; var "y"] |}
+     ];
+     rule_concls := [
+       {| fact_R := "aunt_uncle"; fact_args := [var "x"; var "y"] |}
+     ] |}.
+
+Definition r_cousin : rule :=
+  {| rule_agg := None;
+     rule_hyps := [
+       {| fact_R := "parent"; fact_args := [var "px"; var "x"] |};
+       {| fact_R := "parent"; fact_args := [var "py"; var "y"] |};
+       {| fact_R := "sibling"; fact_args := [var "px"; var "py"] |}
+     ];
+     rule_concls := [
+       {| fact_R := "cousin"; fact_args := [var "x"; var "y"] |}
+     ] |}.
+
+Definition r_bob_parent : rule :=
+  {| rule_agg := None;
+     rule_hyps := [
+       {| fact_R := "parent"; fact_args := [const "Bob"; var "x"] |}
+     ];
+     rule_concls := [
+       {| fact_R := "parent"; fact_args := [const "Bob"; const "Charlie"] |}
+     ] |}.
+
+Definition family_program := 
+  [r_parent_anna;
+   r_ancestor1;
+   r_ancestor2;
+   r_sibling;
+   r_aunt_uncle;
+   r_cousin;
+   r_bob_parent].
+
+Compute get_rule_dependencies family_program r_cousin.
